improved proof setup for swap-correctness (add globel AST def); abstract out swap as in list with abstract relation

backend/Schedulingproof.v
@@ -1,6 +1,6 @@
 
 Require Import Coqlib Maps BoolEqual.
-Require Import AST Integers Values Events Memory Globalenvs Smallstep.
+Require Import AST Integers Values Events Memory Linking Globalenvs Smallstep.
 Require Import Op Locations Conventions Machregs.
 Require Import Mach.
 
@@ -47,47 +47,47 @@ Definition get_srcs (i: instruction): list mreg :=
     end. 
 
 (* register i2 write r, i1 read [..., r, ...]  *)
-Definition data_depends_rw (i1 i2: instruction):=
+Definition happens_before_rw (i1 i2: instruction):=
     match get_srcs i1, get_dst i2 with 
     | srcs, Some dst => mregs_in_list srcs dst
     | _, _ => false
     end.
 
-Definition data_depends_ww (i1 i2: instruction) :=
+Definition happens_before_ww (i1 i2: instruction) :=
     match get_dst i1, get_dst i2 with 
     | Some dst1, Some dst2 => 
         if mreg_eq dst1 dst2 then true else false
     | _, _ => false
     end.
 
-Definition data_depends_mem (i1 i2: instruction):=
+Definition happens_before_mem (i1 i2: instruction):=
     match mem_write i1, mem_write i2 with
     | Some true, Some _ | Some _, Some true => true 
     | _, _ => false
     end.
 
 (* i1 i2 have dependence, order irrelevent *)
-Definition data_depends (i1 i2: instruction): bool :=
+Definition happens_before (i1 i2: instruction): bool :=
     (* solid dependence from control inst. like function calls, return, etc. *)
     if solid_inst i1 then true
     else if solid_inst i2 then true
     (* register dependence *)
-    else if data_depends_rw i1 i2 then true
-    else if data_depends_rw i2 i1 then true
-    else if data_depends_ww i1 i2 then true
+    else if happens_before_rw i1 i2 then true
+    else if happens_before_rw i2 i1 then true
+    else if happens_before_ww i1 i2 then true
     (* memory dependence without alias information 
         - any two memory access with at least write are regarded to have dependence *)
-    else if data_depends_mem i1 i2 then true
+    else if happens_before_mem i1 i2 then true
     (* no dependence *)
     else false.
 
-Notation "i2 <~D~> i1":= (data_depends i1 i2) (at level 1).
+Notation "i1 D~> i2":= (happens_before i1 i2) (at level 1).
 
-Lemma data_depends_inv: 
-    forall i1 i2, data_depends i1 i2 = false ->
+Lemma happens_before_inv_false: 
+    forall i1 i2, happens_before i1 i2 = false ->
         True.
 Proof. auto. Qed.
-    
+
 
 (** topo order from deta independence *)
 Parameter GraphType: Type.
@@ -95,25 +95,85 @@ Fixpoint topo_calcu (bb: list instruction): GraphType. Admitted.
 
 (** swap some pair of consecutive inst. in code *)
 (* note that those are not actual functions that will be used in compiling, but only in correctness proof *)
-Fixpoint try_swap_nth_code (n: nat) (l: list instruction): list instruction:=
+
+(* Fixpoint try_swap_nth_code_aux (n: nat) (l: list instruction): option (list instruction):=
   match n, l with
-  | _, nil => nil
-  | _, i :: nil => i :: nil
-  | O, i1 :: i2 :: l' => if data_depends i1 i2 then l
-                         else i2 :: i1 :: l'
-  | Datatypes.S n', i :: l' => try_swap_nth_code n' l'
-  end.  
+  | _, nil => None | _, i :: nil => None        (* None: did not swap *)
+  | O, i1 :: i2 :: l' => if happens_before i1 i2 then None
+                         else Some (i2 :: i1 :: l')
+  | Datatypes.S n', i :: l' => try_swap_nth_code_aux n' l'
+  end.   *)
+Require Import RelationClasses.
+Section SWAP_ONE_PAIR.
+  Open Scope nat_scope.
+  Context {A: Type}.
+  Variable (rel: A -> A -> bool).
+
+  Fixpoint try_swap (n: nat) (l: list A): list A :=
+    match n, l with
+    | _, nil => nil | _, i :: nil => l        (* None: did not swap *)
+    | O, i1 :: i2 :: l' => if rel i1 i2 then l
+                            else (i2 :: i1 :: l')
+    | Datatypes.S n', i :: l' => try_swap n' l'
+    end. 
+
+    Lemma try_swap_rm_head: 
+      forall (n:nat) l a, 0 < n -> try_swap n (a :: l) = a :: try_swap (n-1) l.
+    Proof. Admitted.
+  
+    Lemma try_swap_at_tail: forall l, try_swap (length l) l = l.
+    Proof.
+      assert(try_swap_at_tail_aux: forall l a, 
+        try_swap (length (a::l)) (a::l) = a :: try_swap (length l) l ).
+      { intros l. induction l; intros. simpl; auto. rewrite  IHl. 
+        admit. (* TODO not a problem; need to reason about length *) 
+      }
+      induction l. simpl; auto.
+      rewrite try_swap_at_tail_aux. rewrite IHl; auto.
+    Admitted.
+
+    Section DECIDE_REL.
+      Variable (Rel: A -> A -> Prop).
+      Hypothesis decide_rel: forall a1 a2, Rel a1 a2 <-> rel a1 a2 = true.
+      
+      (* Hypothesis porder: PartialOrder (@eq A) Rel. *)
+    End DECIDE_REL.
+End SWAP_ONE_PAIR.
+
+
+Definition try_swap_code:= try_swap happens_before.
+  (* match n, l with
+  | _, nil => nil | _, i :: nil => l        (* None: did not swap *)
+  | O, i1 :: i2 :: l' => if happens_before i1 i2 then l
+                          else (i2 :: i1 :: l')
+  | Datatypes.S n', i :: l' => try_swap_code n' l'
+  end.   *)
 
 Definition try_swap_nth_func (n: nat)(f: function):= 
-    mkfunction f.(fn_sig) (try_swap_nth_code n f.(fn_code)) 
+    mkfunction f.(fn_sig) (try_swap_code n f.(fn_code)) 
                f.(fn_stacksize) f.(fn_link_ofs) f.(fn_retaddr_ofs).
 
+(* Fixpoint try_swap_multi_code_aux (ln: list nat) (l: list instruction): option (list instruction) :=
+match ln with
+| nil => None 
+| n :: ln' => match try_swap_nth_code_aux n l with
+                | Some l' => try_swap_multi_code_aux ln' l'
+                | None => None
+                end
+end.
+
+Definition try_swap_multi_code (ln: list nat) (l: list instruction): list instruction :=
+match try_swap_multi_code_aux ln l with
+| Some l' => l'
+| None => l 
+end. *)
+
 (** a consecutive swap *)
-Fixpoint try_swap_n_times (ln: list nat)(f: function) :=
+(* Fixpoint try_swap_multi_func (ln: list nat)(f: function) :=
   match ln with
   | nil => f
-  | n :: ln' => try_swap_n_times ln' (try_swap_nth_func n f)
-  end.
+  | n :: ln' => try_swap_multi_func ln' (try_swap_nth_func n f)
+  end. *)
 
 Require Import Errors.
 Open Scope error_monad_scope.
@@ -123,32 +183,83 @@ Open Scope list_scope.
 Definition transf_function_try_swap_nth (n: nat) (f: function) : res function :=
     OK (try_swap_nth_func n f).
 
-Definition transf_fundef_try_swap_nth (n: nat) (f: fundef) : res fundef :=
-    AST.transf_partial_fundef (transf_function_try_swap_nth n) f.
-Check transform_partial_program.
+Definition transf_fundef_try_swap_nth (n: nat) (f: fundef) : res fundef :=  
+  AST.transf_partial_fundef (transf_function_try_swap_nth n) f.
 
-Definition transf_program_try_swap_nth_in_one (n: nat) (funid: ident) (p: Mach.program): res program :=
-    transform_partial_program2 
-      (fun i f => if ident_eq i funid then transf_fundef_try_swap_nth n f else OK f) 
-      (fun i v => OK v) p.
+(** only swap one independent pair in one function *)
+Definition transf_program_try_swap_nth_in_one (funid: ident) (n: nat) (p: program): res program :=
+  transform_partial_program2 
+  (fun i f => if ident_eq i funid then transf_fundef_try_swap_nth n f else OK f) 
+  (fun i v => OK v) p.
 
-Inductive match_stackframes: stackframe -> stackframe -> Prop :=
-  | match_stackframes_swapped_code:
+Fixpoint transf_program_try_swap_multi_in_one (funid: ident) (ln: list nat)(p: program): res program :=
+  match ln with
+  | nil => OK p
+  | n :: ln' => do p' <- transf_program_try_swap_nth_in_one funid n p;
+                transf_program_try_swap_multi_in_one funid ln' p'
+  end.
+
+Fixpoint transf_program_try_swap_multi_in_multi (pairs:list (ident * list nat))(p:program): res program:=
+  match pairs with
+  | nil => OK p
+  | (funid, ln) :: pairs' => 
+    do p' <- transf_program_try_swap_multi_in_one funid ln p;
+    transf_program_try_swap_multi_in_multi pairs' p  
+  end.
+
+(* Section SIMULATION_FRAMEWORK.
+  
+  Variable real_transf_fundef: fundef -> res fundef.
+  Variable real_transf_program: program -> res program.
+  Hypothesis real_transf_fundef_equiv: True.
+
+  Definition real_match_prog (prog tprog: program) :=
+    match_program (fun ctx f tf => real_transf_fundef f = OK tf) eq prog tprog.
+
+  Section SIMULATION_TRANS.
+    Variable return_address_offset: function -> code -> ptrofs -> Prop.
+    Variable prog: program.
+    Variable tprog: program.
+    Hypothesis TRANSF: real_transf_program prog = OK tprog.
+    Lemma REAL_MATCH_PROG: real_match_prog prog tprog.
+    Proof. unfold real_match_prog, match_program. Admitted.
+    Let ge := Genv.globalenv prog.
+    Let tge := Genv.globalenv tprog.
+
+    Variable pairs: list (ident * list nat).
+    Hypothesis real_trasf_equiv: True.
+   
+    Theorem forward_simulation_transformed:
+      forward_simulation (Mach.semantics return_address_offset prog) 
+                         (Mach.semantics return_address_offset tprog).
+    Proof. unfold real_match_prog, match_program, match_program_gen in TRANSF. Admitted.
+
+  End SIMULATION_TRANS.
+
+  (* Hypothesis real_transf_equiv:
+    forall p, exists pairs, 
+      real_transf p = transf_program_try_swap_multi_in_multi pairs p.
+   *)
+  Variable (pairs:list (ident * list nat)).
+End SIMULATION_FRAMEWORK. *)
+
+Inductive match_stackframe: stackframe -> stackframe -> Prop :=
+  | match_stackframes_intro:
       forall f f' sp sp' ra ra' m c c'
       (FUNC: f = f') 
       (SP: sp = sp') (RA: ra = ra') 
-      (CODE: try_swap_nth_code m c = c'),
-      match_stackframes (Stackframe f sp ra c)
-                        (Stackframe f' sp' ra' c')
+      (CODE: try_swap_code m c = c'),
+      match_stackframe (Stackframe f sp ra c)
+                       (Stackframe f' sp' ra' c')
 .
-Definition match_stack := Forall2 match_stackframes.
+Definition match_stack := Forall2 match_stackframe.
 
 Inductive match_states: state -> state -> Prop :=
   | match_regular_states: 
       forall sl sl' f f' sp sp' n c c' rs rs' m m'
       (STK: match_stack sl sl')
       (FUNC: f = f') (SP: sp = sp')
-      (CODE: try_swap_nth_code n c = c' )
+      (CODE: try_swap_code n c = c' )
       (RS: rs = rs') (MEM: m = m'),
       match_states (State sl f sp c rs m)
                    (State sl' f' sp' c' rs' m')
@@ -168,84 +279,137 @@ Inductive match_states: state -> state -> Prop :=
       match_states (Returnstate sl rs m)
                    (Returnstate sl' rs' m')
 .
-
+Lemma match_stack_refl: forall stk, match_stackframe stk stk.
+Proof. 
+  intros. destruct stk. eapply match_stackframes_intro; auto. 
+  eapply try_swap_at_tail.
+Qed.
 
 (** Correctness proof of general correctness of instruction scheduling algorithm*)
 
+(** Step 1: prove the correctness of one single swap *)
 
-(** Step 1: prove the correctness of simpl swap *)
-Section TWO_STEP_CORRECTNESS.
+Definition match_prog (funid: ident) (n: nat) (p tp: program) :=
+  match_program (fun _ f tf => transf_fundef_try_swap_nth n f = OK tf) eq p tp.
 
-Variable prog: program.
-Variable tprog: program.
-Variable return_address_offset: function -> code -> ptrofs -> Prop.
+Section SINGLE_SWAP_CORRECTNESS.
 
-Let step := step return_address_offset.
+  Variable prog: program.
+  Variable tprog: program.
+  Variable return_address_offset: function -> code -> ptrofs -> Prop.
+  
+  (* only try to swap at one pair inside one function *)
+  Variable funid: ident.
+  Variable n: nat.
+  (* Hypothesis TRANSF: match_prog prog tprog. *)
+  Hypothesis TRANSF_PROG: transf_program_try_swap_nth_in_one funid n prog = OK tprog.
+  Let step := step return_address_offset.
 
-(* Hypothesis TRANSF: match_prog prog tprog. *)
+  Let ge := Genv.globalenv prog.
+  Let tge := Genv.globalenv tprog.
 
-Let ge := Genv.globalenv prog.
-Let tge := Genv.globalenv tprog.
+  Let transf_fun := (fun i f => if ident_eq i funid then transf_fundef_try_swap_nth n f else OK f).
+  Let transf_var := (fun (i: ident) (v:unit) => OK v).
 
-Lemma independ_two_step_match:
-    forall stk1 stk1' f sp bb rs1 m1
-    s1 s3 s1' s3' i1 i2 t t'
-    (INDEP: data_depends i1 i2 = false)
-    (S1: s1 = State stk1 f sp (i1::i2::bb) rs1 m1)
-    (STEP13: starN step ge 2 s1 t s3)
-    (S1': s1' = State stk1' f sp (i2::i1::bb) rs1 m1)
-    (MATCH: match_stack stk1 stk1')
-    (STEP13': starN step ge 2 s1' t' s3'),
-        match_states s3 s3' .
-Proof.
-    intros.
-    inv STEP13. rename s' into s2. inv H1. inv H3. rename t0 into t2.
-    inv STEP13'. rename s' into s2'. inv H3. inv H5. rename t0 into t1'. rename t4 into t2'.
+  Inductive match_fundef (p: program): fundef -> fundef -> Prop :=
+    | match_fundef_same: forall f tf, match_fundef p f tf  
+    | match_fundef_swap_nth: forall n f,
+        match_fundef p (Internal f) (Internal (try_swap_nth_func n f))
+  .
+  Definition match_varinfo: unit -> unit -> Prop := eq.
+  
+  Lemma TRANSF: match_program_gen match_fundef match_varinfo prog prog tprog.
+  Proof. 
+    eapply match_transform_partial_program2. eapply TRANSF_PROG.
+    2: { intros. simpl in H. inv H; apply eq_refl. }
+    intros. simpl in H. destruct (ident_eq).
+    - destruct f; inv H.
+      apply match_fundef_swap_nth. apply match_fundef_same.
+    - inv H; apply match_fundef_same.
+  Qed.
 
-    inv H0.
-    - inv H1; unfold data_depends in INDEP; simpl in INDEP.
-        + inv H2. inv H4. split; auto. 
-        (* apply match_same_locset.
-        intros. Search loc.
-        Print loc. Print slot.
-            Print Locations.Locmap.set.
-            admit.
-        +  admit.
-        + admit.
-        + unfold data_depends_rw in INDEP; simpl in INDEP.
-        remember (mreg_eqb res src) as b; destruct (b); inv INDEP.
-        assert(REGeq: res <> src).
-            intro. rewrite H in Heqb. rewrite mreg_eqb_refl in Heqb. inv Heqb.
-        split. Focus 2.
-        apply match_local_block. *)
-      
-Admitted.
+  (** Note: linking was not supported at current time 
+      because it requires "Level B Correctness" of SepCompCert@POPL'16
+      which is not ported into the CompCert 3.12 code base. 
+      We still prove follow the CompCert 2.6 framework for now *)
 
-Lemma transf_initial_states:
-  forall st1, initial_state prog st1 ->
-  exists st2, initial_state tprog st2 /\ match_states st1 st2.
-Proof. 
-    intros. inv H.
-    exists (Callstate [] fb (Regmap.init Vundef) m0).
-    split.
-    - apply initial_state_intro.
-        (* apply (Genv.init_mem_transf_partial TRANSF); trivial. 
-        rewrite (match_program_main TRANSF).
-        rewrite symbols_preserved; auto. 
-    - apply match_call; auto. *)
-Admitted.
+  Lemma symbols_preserved:
+    forall (s: ident), Genv.find_symbol tge s = Genv.find_symbol ge s.
+  Proof (Genv.find_symbol_match TRANSF). 
 
-Lemma transf_final_states:
-  forall st1 st2 r,
-  match_states st1 st2 -> final_state st1 r -> final_state st2 r.
-Proof. 
-  (* intros. inv H0. inv H. 
-  eapply final_state_intro.
-  eapply H1. trivial. *)
-Admitted.
+  Lemma senv_preserved:
+    Senv.equiv ge tge.
+  Proof (Genv.senv_match TRANSF).
 
-End TWO_STEP_CORRECTNESS.
+  Lemma independ_two_step_match:
+      forall stk1 stk1' f sp bb rs1 m1
+      s1 s3 s1' s3' i1 i2 t t'
+      (INDEP: happens_before i1 i2 = false)
+      (S1: s1 = State stk1 f sp (i1::i2::bb) rs1 m1)
+      (STEP13: starN step ge 2 s1 t s3)
+      (S1': s1' = State stk1' f sp (i2::i1::bb) rs1 m1)
+      (MATCH: match_stack stk1 stk1')
+      (STEP13': starN step ge 2 s1' t' s3'),
+          match_states s3 s3' .
+  Proof.
+      intros.
+      inv STEP13. rename s' into s2. inv H1. inv H3. rename t0 into t2.
+      inv STEP13'. rename s' into s2'. inv H3. inv H5. rename t0 into t1'. rename t4 into t2'.
 
+      inv H0.
+      - inv H1; unfold happens_before in INDEP; simpl in INDEP.
+          (* + inv H2. inv H4. split; auto.  *)
+          (* apply match_same_locset.
+          intros. Search loc.
+          Print loc. Print slot.
+              Print Locations.Locmap.set.
+              admit.
+          +  admit.
+          + admit.
+          + unfold data_depends_rw in INDEP; simpl in INDEP.
+          remember (mreg_eqb res src) as b; destruct (b); inv INDEP.
+          assert(REGeq: res <> src).
+              intro. rewrite H in Heqb. rewrite mreg_eqb_refl in Heqb. inv Heqb.
+          split. Focus 2.
+          apply match_local_block. *)
+        
+  Admitted.
+
+  Lemma transf_initial_states:
+    forall st1, initial_state prog st1 ->
+    exists st2, initial_state tprog st2 /\ match_states st1 st2.
+  Proof. 
+      intros. inv H.
+      exists (Callstate [] fb (Regmap.init Vundef) m0).
+      split.
+      - apply initial_state_intro.
+          apply (Genv.init_mem_match TRANSF); trivial. 
+          rewrite (match_program_main TRANSF).
+          rewrite symbols_preserved; auto. 
+      - apply match_callstate; auto. apply Forall2_nil.
+  Qed.
+
+  Lemma transf_final_states:
+    forall st1 st2 r,
+    match_states st1 st2 -> final_state st1 r -> final_state st2 r.
+  Proof. 
+    intros. inv H0. inv H. inv STL.
+    eapply final_state_intro.
+    eapply H1. trivial.
+  Qed.
+  
+  Theorem forward_simulation_transformed:
+  forward_simulation (Mach.semantics return_address_offset prog) 
+                     (Mach.semantics return_address_offset tprog).
+  Proof.
+    eapply forward_simulation_star.
+    - apply senv_preserved.
+    - apply transf_initial_states.
+    - apply transf_final_states.
+    -
+  Admitted.
+
+End SINGLE_SWAP_CORRECTNESS.
 
 Section SWAP_CORRECT_TO_SCHEDULING_CORRECT.
 
@@ -305,7 +469,38 @@ Definition transf_program (p: Mach.program) : res program :=
 
 
 
+    Section GENV_2_6.
 
+    Variable A B V W: Type.
+    Variable transf_fun: ident -> A -> res B.
+    Variable transf_var: ident -> V -> res W.
+    Variable p: AST.program A V.
+    Variable p': AST.program B W.
+    Hypothesis transf_OK:
+      transform_partial_program2 transf_fun transf_var p = OK p'.
+    
+    (* Remark transf_augment_OK:
+      transform_partial_augment_program transf_fun transf_var nil p.(prog_main) p = OK p'.
+    Proof.
+      rewrite <- transf_OK. symmetry. apply transform_partial_program2_augment.
+    Qed. *)
+    End GENV_2_6.
+    
+    (** Extension from Globleenvs.v *)
+    Section GENV_EXT.
+        Section TRANSF_PROGRAM_EXT.
+    
+        Context {A B V: Type}.
+        Variable transf_fun: ident -> A -> B.
+    
+        Definition transf_globdef (idg: ident * globdef A V) : ident * globdef B V :=
+            match idg with
+            | (id, Gfun f) => (id, Gfun (transf_fun id f))
+            | (id, Gvar v) => (id, Gvar v)
+            end.
+    
+        End TRANSF_PROGRAM_EXT.
+    End GENV_EXT.
 
 
 
